src/hls/GibleSeqgen.v
@@ -1,0 +1,153 @@
+(*|
+..
+   Vericert: Verified high-level synthesis.
+   Copyright (C) 2020-2022 Yann Herklotz <yann@yannherklotz.com>
+
+   This program is free software: you can redistribute it and/or modify
+   it under the terms of the GNU General Public License as published by
+   the Free Software Foundation, either version 3 of the License, or
+   (at your option) any later version.
+
+   This program is distributed in the hope that it will be useful,
+   but WITHOUT ANY WARRANTY; without even the implied warranty of
+   MERCHANTABILITY or FITNESS FOR A PARTICULAR PURPOSE.  See the
+   GNU General Public License for more details.
+
+   You should have received a copy of the GNU General Public License
+   along with this program.  If not, see <https://www.gnu.org/licenses/>.
+
+===========
+RTLBlockgen
+===========
+
+.. coq:: none
+|*)
+
+Require compcert.backend.RTL.
+Require Import compcert.common.AST.
+Require Import compcert.lib.Maps.
+Require Import compcert.lib.Integers.
+Require Import compcert.lib.Floats.
+
+Require Import vericert.common.DecEq.
+Require Import vericert.common.Vericertlib.
+Require Import vericert.hls.Gible.
+Require Import vericert.hls.GibleSeq.
+
+#[local] Open Scope positive.
+
+Definition check_valid_node (tc: code) (e: node) :=
+  match tc ! e with
+  | Some _ => true
+  | _ => false
+  end.
+
+Fixpoint check_code (c: RTL.code) (tc: code) (pc: node) (b: BB.t) :=
+  match c ! pc, b with
+  | Some (RTL.Inop pc'), RBnop :: (_ :: _ :: _) as b' =>
+      check_code c tc pc' b'
+  | Some (RTL.Iop op' args' dst' pc'), RBop None op args dst :: (_ :: _ :: _) as b' =>
+      ceq operation_eq op op'
+      && ceq list_pos_eq args args'
+      && ceq peq dst dst'
+      && check_code c tc pc' b'
+  | Some (RTL.Iload chunk' addr' args' dst' pc'),
+    RBload None chunk addr args dst :: (_ :: _ :: _) as b' =>
+      ceq memory_chunk_eq chunk chunk'
+      && ceq addressing_eq addr addr'
+      && ceq list_pos_eq args args'
+      && ceq peq dst dst'
+      && check_code c tc pc' b'
+  | Some (RTL.Istore chunk' addr' args' src' pc'),
+    RBstore None chunk addr args src :: (_ :: _ :: _) as b' =>
+      ceq memory_chunk_eq chunk chunk'
+      && ceq addressing_eq addr addr'
+      && ceq list_pos_eq args args'
+      && ceq peq src src'
+      && check_code c tc pc' b'
+  | Some (RTL.Inop pc''), RBnop :: RBexit None (RBgoto pc') :: nil =>
+      check_valid_node tc pc'
+      && ceq peq pc' pc''
+  | Some (RTL.Iop op' args' dst' pc''), RBop None op args dst :: RBexit None (RBgoto pc') :: nil =>
+      check_valid_node tc pc'
+      && ceq peq pc' pc''
+      && ceq operation_eq op op'
+      && ceq list_pos_eq args args'
+      && ceq peq dst dst'
+  | Some (RTL.Iload chunk' addr' args' dst' pc''),
+    RBload None chunk addr args dst :: RBexit None (RBgoto pc') :: nil =>
+      check_valid_node tc pc'
+      && ceq peq pc' pc''
+      && ceq memory_chunk_eq chunk chunk'
+      && ceq addressing_eq addr addr'
+      && ceq list_pos_eq args args'
+      && ceq peq dst dst'
+  | Some (RTL.Istore chunk' addr' args' src' pc''),
+    RBstore None chunk addr args src :: RBexit None (RBgoto pc') :: nil =>
+      check_valid_node tc pc'
+      && ceq peq pc' pc''
+      && ceq memory_chunk_eq chunk chunk'
+      && ceq addressing_eq addr addr'
+      && ceq list_pos_eq args args'
+      && ceq peq src src'
+  | Some (RTL.Icall sig' (inl r') args' dst' pc''),
+    RBnop :: RBexit None (RBcall sig (inl r) args dst pc') :: nil =>
+      check_valid_node tc pc'
+      && ceq peq pc' pc''
+      && ceq signature_eq sig sig'
+      && ceq peq r r'
+      && ceq list_pos_eq args args'
+      && ceq peq dst dst'
+  | Some (RTL.Icall sig' (inr i') args' dst' pc''),
+    RBnop :: RBexit None (RBcall sig (inr i) args dst pc') :: nil =>
+      check_valid_node tc pc'
+      && ceq peq pc' pc''
+      && ceq signature_eq sig sig'
+      && ceq peq i i'
+      && ceq list_pos_eq args args'
+      && ceq peq dst dst'
+  | Some (RTL.Itailcall sig (inl r) args),
+    RBnop :: RBexit None (RBtailcall sig' (inl r') args') :: nil =>
+      ceq signature_eq sig sig'
+      && ceq peq r r'
+      && ceq list_pos_eq args args'
+  | Some (RTL.Itailcall sig (inr r) args),
+    RBnop :: RBexit None (RBtailcall sig' (inr r') args') :: nil =>
+      ceq signature_eq sig sig'
+      && ceq peq r r'
+      && ceq list_pos_eq args args'
+  | Some (RTL.Icond cond args n1 n2), RBnop :: RBexit None (RBcond cond' args' n1' n2') :: nil =>
+      check_valid_node tc n1
+      && check_valid_node tc n2
+      && ceq condition_eq cond cond'
+      && ceq list_pos_eq args args'
+      && ceq peq n1 n1'
+      && ceq peq n2 n2'
+  | Some (RTL.Ijumptable r ns), RBnop :: RBexit None (RBjumptable r' ns') :: nil =>
+      ceq peq r r'
+      && ceq list_pos_eq ns ns'
+      && forallb (check_valid_node tc) ns
+  | Some (RTL.Ireturn (Some r)), RBnop :: RBexit None (RBreturn (Some r')) :: nil =>
+      ceq peq r r'
+  | Some (RTL.Ireturn None), RBnop :: RBexit None (RBreturn None) :: nil => true
+  | _, _ => false
+  end.
+
+Parameter partition : RTL.function -> Errors.res function.
+
+Definition transl_function (f: RTL.function) :=
+  match partition f with
+  | Errors.OK f' =>
+      if check_valid_node f'.(fn_code) f.(RTL.fn_entrypoint) then
+        if forall_ptree (check_code f.(RTL.fn_code) f'.(fn_code)) f'.(fn_code) then
+          Errors.OK
+            (mkfunction f.(RTL.fn_sig) f.(RTL.fn_params) f.(RTL.fn_stacksize) f'.(fn_code) f.(RTL.fn_entrypoint))
+        else Errors.Error (Errors.msg "check_present_blocks failed")
+      else Errors.Error (Errors.msg "entrypoint does not exists")
+  | Errors.Error msg => Errors.Error msg
+  end.
+
+Definition transl_fundef := transf_partial_fundef transl_function.
+
+Definition transl_program : RTL.program -> Errors.res program :=
+  transform_partial_program transl_fundef.
